src/basic/FStarC.Errors.Codes.fsti
@@ -398,6 +398,8 @@ type error_code =
   | Warning_CustardIneffectiveAttribute
   | Error_CustardNotCompileTime
   | Warning_CustardKeyNotReduced
+  | Error_CustardExportCollision
+  | Warning_CustardNoPublicDefinitions
   | Error_AmbiguousName
 
 type error_setting = error_code & error_flag & int
